#+TITLE: Section 2: Light Quantization
#+LATEX_COMPILER: xelatex
#+LATEX_CLASS_OPTIONS: [12pt]
#+LATEX_HEADER: \usepackage[b5paper, landscape, margin=1in]{geometry}

* Light in a 1D cavity
Because the wave equation is a linear equation, we are able to employ the
quasi-1D approximation and only consider one mode of the light propagate along
one direction with polarization along another direction. If the system we are facing
requires more complicate wave, we can build it from the simple condition we
considered here, which is guaranteed by the orthogonality between the modes and
between the different directions.

#+CAPTION: Real cavity
#+ATTR_LATEX: :width 2in :float
#+ATTR_HTML: :width 300px
#+ATTR_ORG: :width 300
[[../figs/real_optical_cavity.png]]
#+CAPTION: 1D cavity
#+ATTR_LATEX: :width 3in :float
#+ATTR_HTML: :width 600px
#+ATTR_ORG: :width 600px
[[../figs/1d-cavity.png]]

The formal solution of mode $k$ of the light which propagates along the z
direction with polarization along x direction is
\begin{equation}
\vec{A} = \hat{e}_{x}\pqty{A_{k}q_{k}(t)e^{ikz}+A_{-k}q_{-k}(t)e^{-ikz}},
\end{equation}
So,
\begin{equation}
\vec{E} = -\partial_{t}\vec{A} = -\hat{e}_{x}\pqty{A_{k}\dot{q}_{k}(t)e^{ikz}+A_{-k}\dot{q}_{-k}(t)e^{-ikz}},
\end{equation}
\begin{equation}
\vec{B} = \vec{\nabla}\times\vec{A} = -\hat{e}_{y} \pqty{A_{k}kq_{k}(t)e^{ikz}-A_{-k}kq_{-k}(t)e^{-ikz}}.
\end{equation}

A simple 1D-cavity consisting on two perfectly conducting plane mirrors facing
each other. Light propagate between the mirrors back and forth which implies
\begin{equation}
A_{k} = A_{-k}.
\end{equation}

The components of the electric field parallel to the conducting mirrors must
vanish. Taking $z=0$ at the mirror on the left and $z=L$ at the mirror on the
right.

The $z=0$ boundary condidtions imply
\begin{equation}
\vec{E}(0,t) = 0 \Rightarrow A_{k}\dot{q}_{k}(t) = - A_{-k}\dot{q}_{-k}(t) \Rightarrow q_{k}(t) = -q_{-k}(t).
\end{equation}

The $z=L$ boundary condidtions imply
\begin{equation}
\begin{split}
&\vec{E}(L,t) = 0 \Rightarrow A_{k}\dot{q}_{k}(t)e^{ikL} = - A_{-k}\dot{q}_{-k}(t)e^{-ikL} \\
\Rightarrow\ &e^{ikL}+e^{-ikL} = i\sin(kL) = 0 \\
\Rightarrow\ &k = \frac{n\pi}{L}, \qq{with} n\in N. \\
\end{split}
\end{equation}

Now we have formal solution
\begin{equation}
\vec{A} = \vec{e}_{x} A_{n}q_{n}(t)\sin(k_{n}z),
\end{equation}
\begin{equation}
\vec{E} = -\vec{e}_{x} A_{n}\dot{q}_{n}(t)\sin(k_{n}z),
\end{equation}
\begin{equation}
\vec{B} = \vec{e}_{y} k_{n}A_{n}q_{n}(t)\cos(k_{n}z),
\end{equation}
with $k_{n} = n\pi/L$, $n=1, 2, 3,\dots$.

Using the expression above, we calculate the electromagnetc energy as follows
\begin{equation}
\begin{split}
\ &E_{\text{em}}(t) \\
=\ &\frac{1}{2} \int_{\mathrm{cavity}} \dd^{3}\vec{r} \pqty{\varepsilon_{0}\vec{E}^{2}(z,t) + \frac{1}{\mu_{0}}\vec{B}^{2}(z,t)} \\
=\ &\small{\frac{1}{2} \int_{\mathrm{cavity}}\dd x\dd y \cdot A_{n}^{2} \pqty{\varepsilon_{0}\dot{q}_{n}^{2}(t)\int_{0}^{L}\dd z \sin^{2}(k_{n}z) + \frac{k_{n}^{2}}{\mu_{0}}q^{2}_{n}(t)\int_{0}^{L}\dd z \cos^{2}(k_{n}z)}} \\
=\ &\frac{\varepsilon_{0} LS}{4}A_{n}^{2}\pqty{\dot{q}_{n}^{2}(t)+c^{2}k_{n}^{2}q_{n}^{2}(t)},
\end{split}
\end{equation}
in which, we use the mathematical relation
\begin{equation}
\int_{0}^{L}\dd z\sin(k_{n}z)\sin(k_{m}z) = \int_{0}^{L}\dd z \cos(k_{n}z)\cos(k_{m}z) = \frac{L}{2}\delta_{nm}.
\end{equation}

In fact, if we choose more general formal solution $\vec{A} = \hat{e}_{x}\sum_{n=1}^{\infty}A_{n}q_{n}(t)\sin(k_{n}z)$, we will arrive the same
place,
\begin{equation}
\begin{split}
\ &E_{\text{em}}(t) \\
=\ &\frac{1}{2} \int_{\mathrm{cavity}} \dd^{3}\vec{r} \pqty{\varepsilon_{0}\vec{E}^{2}(z,t) + \frac{1}{\mu_{0}}\vec{B}^{2}(z,t)} \\
=\ &\small{\frac{1}{2} \int_{\mathrm{cavity}}\dd x\dd y \cdot \sum_{n,m=1}^{\infty}A_{n}A_{m}\pqty{\varepsilon_{0}\dot{q}_{n}(t)\dot{q}_{m}(t)\int_{0}^{L}\dd z \sin(k_{n}z)\sin(k_{m}z) + \frac{k_{n}k_{m}}{\mu_{0}}q_{n}(t)q_{m}(t)\int_{0}^{L}\dd z \cos(k_{n}z)\cos(k_{m}z)}} \\
=\ &\frac{\varepsilon_{0} LS}{4}\sum_{n=1}^{\infty}A_{n}^{2}\pqty{\dot{q}_{n}^{2}(t)+c^{2}k_{n}^{2}q_{n}^{2}(t)},
\end{split}
\end{equation}
in which, the $\sin(k_{n}z)\sin(k_{m}z)$ term equals to zero due to the
orthogonal relation.

If we choose $A_{n}^{2} = 2m_{n}/\varepsilon_{0}LS$, we have
\begin{equation}
E_{\mathrm{em}}(t) = \sum_{n=1}^{\infty}\bqty{\frac{p_{n}^{2}(t)}{2m_{n}} + \frac{m_{n}\omega_{n}^{2}}{2}q_{n}^{2}(t)},
\end{equation}
in which $m_{n} = \sqrt{A_{n}^{2}\varepsilon_{0}LS/2}$ and $\omega_{n} = ck_{n}$.

* The quantization of the harmonic oscillator
